Work on EtM with Markulf
We broke the AE.decrypt proof (2 assumes), but the hope is that we can
prove stronger post-condition now.

examples/crypto/EtM.AE.fst
@@ -11,29 +11,17 @@ open EtM
 open Platform.Bytes
 open CoreCrypto
 
-type log_t (r:rid) = Monotonic.Seq.log_t r (CPA.msg * CPA.cipher * MAC.tag)
+type cipher = (CPA.cipher * MAC.tag) 
+
+type log_t (r:rid) = Monotonic.Seq.log_t r (CPA.msg * cipher)
 
 
 noeq type key = 
-  | Key:  #region:rid -> ke:CPA.key { extends (CPA.Key.region ke) region  } -> km:MAC.key { extends (MAC.Key.region km) region /\  (disjoint( CPA.Key.region ke) (MAC.Key.region km)) } -> log:log_t region -> key 
-
-
-let invariant (h:t) (k:key) = 
-  let log = m_sel h k.log in
-  let mac_log = m_sel h (MAC.Key.log k.km) in
-  let cpa_log = m_sel h (CPA.Key.log k.ke) in
-  Map.contains h k.region /\
-  Map.contains h (MAC.Key.region k.km) /\
-  Map.contains h (CPA.Key.region k.ke) /\
-  Seq.length log = Seq.length mac_log /\ 
-  Seq.length mac_log = Seq.length cpa_log /\ 
-  (forall (i:int). indexable log i ==>
-    (let m1,t = Seq.index mac_log i in
-    let m2,c = Seq.index cpa_log i in
-    m1 = c /\
-    Seq.index log i = (m2,c,t) 
-    )
-  )
+  | Key:  #region:rid ->
+               ke:CPA.key { extends (CPA.Key.region ke) region  } ->
+               km:MAC.key { extends (MAC.Key.region km) region /\
+                 (disjoint( CPA.Key.region ke) (MAC.Key.region km)) } ->
+               log:log_t region -> key 
 
 let get_log (h:t) (k:key) = 
   m_sel h k.log
@@ -44,8 +32,24 @@ let get_mac_log (h:t) (k:key) =
 let get_cpa_log (h:t) (k:key) = 
   m_sel h (CPA.Key.log k.ke)
 
+let invariant (h:t) (k:key) = 
+  let log = get_log h k in
+  let mac_log = get_mac_log h k in
+  let cpa_log = get_cpa_log h k in
+  Map.contains h k.region /\
+  Map.contains h (MAC.Key.region k.km) /\
+  Map.contains h (CPA.Key.region k.ke) /\
+  Seq.length log = Seq.length mac_log /\ 
+  Seq.length mac_log = Seq.length cpa_log /\ 
+  (forall (i:int). indexable log i ==>
+    (let m1,t = Seq.index mac_log i in
+     let m2,c = Seq.index cpa_log i in
+     m1 = c /\
+     Seq.index log i = (m2,(c,t))
+    )
+  )
 
-type cipher = (CPA.cipher * MAC.tag) 
+
 
 
 let genPost parent h0 (k:key) h1 =
@@ -65,8 +69,8 @@ val keygen: parent:rid -> ST key
 
 let keygen parent =
   let region = new_region parent in
-  let ke = CPA.gen region in
-  let ka = MAC.gen region in
+  let ke = CPA.keygen region in
+  let ka = MAC.keygen region in
   let log = alloc_mref_seq region createEmpty in
   Key #region ke ka log
 
@@ -76,19 +80,18 @@ val encrypt: k:key -> m:Plain.plain -> ST cipher
   (ensures  (fun h0 c h1 ->
     (let log0 = get_log h0 k in
      let log1 = get_log h1 k in
-     let n = Seq.length log0 in
-       modifies (Set.singleton k.region)  h0 h1
-     /\ log1 == snoc log0 (m, fst c, snd c)
-     /\ witnessed (at_least n (m, fst c, snd c) k.log)
-     /\ (invariant h0 k ==> invariant h1 k))))
+     modifies (Set.singleton k.region)  h0 h1
+     /\ log1 == snoc log0 (m, c)
+     /\ witnessed (at_least (Seq.length log0) (m, c) k.log)
+     /\ invariant h1 k)))
 
 #set-options "--initial_fuel 0 --max_fuel 0 --initial_ifuel 1 --max_ifuel 1 --z3timeout 100"
 let encrypt k plain =
-  let h0 = ST.get () in
+  (* let h0 = ST.get () in *)
   let c = CPA.encrypt k.ke plain in
   let t = MAC.mac k.km c in
-  write_at_end k.log (plain,c,t);
-  let h1 = ST.get () in
+  write_at_end k.log (plain, (c, t));
+  (* let h1 = ST.get () in *)
   //following assertions seem no longer needed
   (* cut (Seq.length (get_log h1 k) = (Seq.length (get_log h0 k)) + 1);   *)
   (* cut (Seq.length (get_mac_log h1 k) = Seq.length (get_cpa_log h1 k)); *)
@@ -96,45 +99,44 @@ let encrypt k plain =
   (* cut (Seq.index (get_mac_log h1 k) (Seq.length (get_mac_log h1 k)-1) = (c,t)); *)
   (* cut (Seq.index (get_cpa_log h1 k) (Seq.length (get_cpa_log h1 k)-1) = (plain,c)); *)
   (* cut (Seq.index (get_log h1 k) (Seq.length (get_log h1 k)-1) = (plain,c,t));  *)
-  assert
-  ( let log  = get_log h1 k in
-    let mac_log = get_mac_log h1 k in
-    let cpa_log = get_cpa_log h1 k in
-    (forall (i:int). indexable log i ==>
-      (let m1,t = Seq.index mac_log i in
-      let m2,c = Seq.index cpa_log i in
-      m1 = c /\
-      Seq.index log i = (m2,c,t) /\
-      True)
-    )
-    );
+  (* assert *)
+  (* ( let log  = get_log h1 k in *)
+  (*   let mac_log = get_mac_log h1 k in *)
+  (*   let cpa_log = get_cpa_log h1 k in *)
+  (*   (forall (i:int). indexable log i ==> *)
+  (*     (let m1,t = Seq.index mac_log i in *)
+  (*     let m2,c = Seq.index cpa_log i in *)
+  (*     m1 = c /\ *)
+  (*     Seq.index log i = (m2,c,t) /\ *)
+  (*     True) *)
+  (*   ) *)
+  (*   ); *)
   (c, t)
-  
 
 //assume AE_needs_CMA: ((b2t Ideal.uf_cma) <==> Ideal.ind_cpa)
 
 val decrypt: k:key -> c:cipher -> ST (option Plain.plain)
   (requires (fun h0 -> invariant h0 k))
-  (ensures (fun h0 p h1 -> 
+  (ensures (fun h0 res h1 -> 
     modifies_none h0 h1 /\ 
-    (invariant h0 k ==> (invariant h1 k /\
-      ( (b2t Ideal.uf_cma /\ is_Some p) ==>
-        ( let log = get_log h0 k in
-          let found = seq_find 
-            (
-              fun (_,c',tag') -> 
-            	  c'= fst c && tag' = snd c
-            ) log in
-          is_Some found /\ 
-          (* ( let Some (p',_,_) = found  in *)
-   	  (*   p = Some(p')  *)
-	  (* ) /\ *)
-	  True
-        )
+    ((invariant h1 k /\
+      ( (b2t Ideal.uf_cma /\ is_Some res) ==>
+        SeqProperties.mem (Some.v res, c) (m_sel h0 k.log)
+        (* (let log = get_log h0 k in *)
+        (*   let found = seq_find  *)
+        (*     ( *)
+        (*       fun (_,c',tag') ->  *)
+        (*     	  c'= fst c && tag' = snd c *)
+        (*     ) log in *)
+        (*   is_Some found /\  *)
+        (*   (\* ( let Some (p',_,_) = found  in *\) *)
+   	(*   (\*   p = Some(p')  *\) *)
+	(*   (\* ) /\ *\) *)
+	(*   True *)
+        (* ) *)
       )
     ))
   ))
-
 
 let decrypt k (c,tag) =
   if MAC.verify k.km c tag
@@ -142,12 +144,18 @@ let decrypt k (c,tag) =
     if (Ideal.uf_cma) then 
       (
       let h = ST.get () in
-      assert ( is_Some (seq_find (fun mt -> mt = (c,tag)) (get_mac_log h k) ) );
+      assert ( SeqProperties.mem (c,tag) (get_mac_log h k) );
+      (* assume ( forall c tag. SeqProperties.mem (c,tag) (get_mac_log h k) ==> *)
+      (*             (exists p. SeqProperties.mem (p,c) (get_cpa_log h k) )); *)
+      (* assert ( exists p. SeqProperties.mem (p,c) (get_cpa_log h k)); *)
+      assume ( is_Some (seq_find (fun mc -> snd mc = c) (get_cpa_log h k) ));
 
       let p = CPA.decrypt k.ke c in
-      assert ( is_Some (seq_find (fun (p',c') -> (p',c') = (p,c)) (get_cpa_log h k) ) );
+      assert ( SeqProperties.mem (p,c) (get_cpa_log h k) );
+      (* assert ( is_Some (seq_find (fun (p',c') -> (p',c') = (p,c)) (get_cpa_log h k) ) ); 
+         -- this one used to work *)
       //assert ( is_Some (seq_find (fun (p',c',tag') -> (p',c',tag') = (p,c,tag)) (get_log h k) ) );
-      (* admit(); *)
+      assume (SeqProperties.mem (p, (c,tag)) (get_log h k));
       Some(p)
       )
     else 
