examples/crypto/EtM.CPA.fst
@@ -17,18 +17,12 @@ open EtM.Plain
 
 type ivsize = blockSize AES_128_CBC
 type keysize = 16
-type aes_key = lbytes keysize
+type aes_key = lbytes keysize (* = b:bytes{B.length b = keysize} *)
 type msg = plain
-type cipher = l:bytes{B.length l >= ivsize}
+type cipher = b:bytes{B.length b >= ivsize}
+(* MK: minimal cipher length twice blocksize? *)
 
 type log_t (r:rid) = Monotonic.Seq.log_t r (msg * cipher)
-
-type corruption_state =
-  | Coerced
-  | Leaked
-  | Open
-  | Private
-
 
 noeq type key =
   | Key: #region:rid -> raw:aes_key -> log:log_t region -> key
@@ -40,53 +34,53 @@ let genPost parent m0 (k:key) m1 =
   /\ m_contains k.log m1
   /\ m_sel m1 k.log == createEmpty
 
-val gen: parent:rid -> ST key
+val keygen: parent:rid -> ST key
   (requires (fun _ -> True))
   (ensures  (genPost parent))
 
-let gen parent =
+let keygen parent =
   let raw = random keysize in
   let region = new_region parent in
   let log = alloc_mref_seq region createEmpty in
   Key #region raw log
 
 val encrypt: k:key -> m:msg -> ST cipher
-  (requires (fun _ -> True))
-  (ensures  (fun m0 c m1 ->
-    (let ilog = m_sel m0 k.log in
-     let n = Seq.length ilog in
-      modifies_one k.region m0 m1 /\
-      m_contains k.log m1
-     /\ m_sel m1 k.log == snoc ilog (m, c)
-     /\ witnessed (at_least n (m, c) k.log))))
+  (requires (fun h0 -> True (* If we wanted to avoid recall:
+                               m_contains k.log h0 *)))
+  (ensures  (fun h0 c h1 ->
+    (let log0 = m_sel h0 k.log in
+     let log1 = m_sel h1 k.log in
+      modifies_one k.region h0 h1 /\
+      m_contains k.log h1
+     /\ log1 == snoc log0 (m, c)
+     /\ witnessed (at_least (Seq.length log0) (m, c) k.log))))
 
 
 let encrypt k m : cipher =
   m_recall k.log;
   let iv = random ivsize in
-  let ilog = m_read k.log in
   let text = if ind_cpa then createBytes (length m) 0z else repr m in
   let c = CoreCrypto.block_encrypt AES_128_CBC k.raw iv text in
   let c = iv@|c in
-  assert(B.length c >= ivsize);
   write_at_end k.log (m,c);
   c
-  
+
 
 val decrypt: k:key -> c:cipher -> ST msg
   (requires (fun h0 ->
     Map.contains h0 k.region /\
-    (let log = m_sel h0 k.log in
-      (b2t ind_cpa_rest_adv) ==> is_Some (seq_find (fun mc -> snd mc = c) log))))
+    (let log0 = m_sel h0 k.log in
+      (b2t ind_cpa_rest_adv) ==> is_Some (seq_find (fun mc -> snd mc = c) log0))))
   (ensures  (fun h0 res h1 ->
     modifies_none h0 h1 /\
-    ( (b2t ind_cpa_rest_adv) ==>
-     (let log = m_sel h0 k.log in
-      let found = seq_find (fun mc -> snd mc = c) log in
-      is_Some found /\ (let Some mc = found in (res,c) = mc)))
+    ( (b2t ind_cpa_rest_adv) ==> SeqProperties.mem (res,c) (m_sel h0 k.log)
+     (* (let log0 = m_sel h0 k.log in *)
+     (*  let found = seq_find (fun mc -> snd mc = c) log0 in *)
+     (*  is_Some found /\ fst (Some.v found) = res) *)
     )
   )
-    
+  )
+
 let decrypt k c =
   if ind_cpa_rest_adv then
     let log = m_read k.log in
