examples/crypto/EtM.Ideal.fsti
@@ -2,9 +2,7 @@ module EtM.Ideal
 
 val ind_cpa : bool
 
-val uf_cma : b:bool{ ind_cpa ==> b}
-
-let priv = ind_cpa
+val uf_cma : b:bool{ ind_cpa ==> b }
 
 let ind_cpa_rest_adv = uf_cma 
 (* well typed adversaries only submit ciphertext obtained using encrypt *)
