examples/crypto/EtM.Plain.fst
@@ -10,10 +10,10 @@ assume Plain_hasEq: hasEq plain
 
 //assume val ind_cpa: bool
 
-val repr: p:plain{~ind_cpa} -> Tot bytes
+val repr: p:plain{not ind_cpa} -> Tot bytes
 let repr p = p
 
-val coerce: r:bytes{(not ind_cpa) || (not uf_cma)} -> Tot plain
+val coerce: r:bytes{not uf_cma} -> Tot plain
 let coerce r = r
 
 val length: plain -> Tot nat
